#+TITLE: Ficha1

* 1.
** a)
*** 1)
\begin{align*}
    &(f . g) x\\
= \{\ &(f.g)x=f(gx) \ (72);\ g(x)=x+1\ (pelo \ enunciado) \ \}\\
    &f(x+1)\\
= \{\ &fx = 2x \ (pelo enunciado) \ \}\\
    &2(x+1)\\
= \{\ &trivial \ \}\\
    &2x+2\\
\end{align*}

*** 2)
\begin{align*}
    &(f . g) x\\
= \{\ &(f.g)x=f(g(x))\ (72);\ g(x)=2x \ \}\\
    &f(2x)\\
= \{\ &fx= succ\ (72)\ \}\\
    &2x + 1
\end{align*}
*** 3)
nao ta feito
*** 4)
\begin{align*}
    &(f.g)x=f(gx)\\
= \{\ &(f.g)x=f(gx)\ (72);\ g(x,y)=x+y\ (pelo\ enunciado) \ \}\\
    &f(x+y)\\
= \{\ &fx=succ(2x) \ \}\\
    &succ(2(x+y))\\
= \{\ &trivial\ \}\\
    &2x+2y+1
\end{align*}
** b)
\begin{align*}
    &((f.g).h)x=f(g(hx))\\
= \{\ &Igualdade\ extensional\ (71) \ \}\\
    &((f.g).h)x=(f(g.h)).x \\
= \{\ &(72)\ Duas\ vezes\ \}\\
    &(f.g)(hx)=f((g.h).x) \\
= \{\ &(72)\ Duas\ vezes\ \}\\
    &f(g(hx))=f(g(hx)) \\
\end{align*}

* 2)
\begin{align*}
    &(f \times g)(fx,gy)=(fx,gy)\\
\\
    &(f \times g)(x,g)\\
\Leftrightarrow \{\ &F_1\ (10)\ do\ formulario \ \}\\
    &<f\circ\pi_1.g\circ\pi_2>(x,y)\\
\Leftrightarrow \{\ &<f.g>=(fx,gy)\ (76)\ \}\\
    &((f\circ\pi_1(x,y)).(g\circ\pi_2(x,y)))\\
\Leftrightarrow \{\ &(72)\ 2\ vezes \ \}\\
    &(f(\pi_1(x,y))\circ(g(\pi_2(x,y))\\
\end{align*}
